\documentclass[a4paper,10pt]{article}
\input{preamble}

%\documentclass[../main.tex]{subfiles}
%\graphicspath{{\subfix{../fig/}}}

\begin{document}

\section{Commensurate Angles}


\begin{figure}[H]
\centering
\includegraphics[width=0.4\textwidth]{fig/latvec.png}
\caption{Commensurate angle case and lattice vectors. Taken from \cite{koshino2012}}
\label{fig:latvec}
\end{figure}

As drawn in Figure \ref{fig:latvec}, we have
\begin{align}
\label{eq:scalarprods1}
\vb{a}_1^{(1)} \vdot \vb{a}_2^{(1)} &= a^2 \cos(60^\circ) = a^2/2; \\
\label{eq:scalarprods2}
\vb{a}_1^{(1)} \vdot \vb{a}_1^{(2)} &= a^2 \cos\theta; \\
\label{eq:scalarprods3}
\vb{a}_1^{(1)} \vdot \vb{a}_2^{(2)} &= a^2 \cos(60^\circ + \theta); \\
\label{eq:scalarprods4}
\vb{a}_1^{(2)} \vdot \vb{a}_2^{(1)} &= a^2 \cos(60^\circ - \theta).
\end{align}

The superlattice vectors $\vb{L}_1$, $\vb{L}_2$ (when the angle is commensurate) are related by a $60^\circ$ rotation. In general, because $\vb{L}_1$ is a point that belongs to the lattices of both layers, it is written by integers $m,n,m',n'$ as
\begin{equation} \label{eq:L1}
\vb{L}_1 = m\vb{a}_1^{(1)} + n\vb{a}_2^{(1)} = m'\vb{a}_1^{(2)} + n'\vb{a}_2^{(2)}.
\end{equation}

Koshino \cite{koshino2012} argues that there is an appropriate choice of lattice vectors $\vb{a}_1^{(1)}, \vb{a}_2^{(1)}, \vb{a}_1^{(2)}, \vb{a}_2^{(2)}$ (satisfying equations \ref{eq:scalarprods1} to \ref{eq:scalarprods4}) such that the indices $(m',n')$ can be made equal to $(n,m)$. If this is true, then by taking the scalar products of equation \ref{eq:L1} with $\vb{a}_1^{(1)}$ and $\vb{a}_1^{(2)}$, we get
$$
\begin{cases}
\; m + n/2 = n \cos\theta + m \cos(60^\circ + \theta); \\
\; m/2 + n = m \cos\theta + n \cos(60^\circ - \theta).
\end{cases}
\Rightarrow
\begin{cases}
\; mn + n^2/2 = n^2 \cos\theta + mn \qty(\frac{\cos\theta}{2}
- \frac{\sqrt{3} \sin\theta}{2}); \\
\; m^2/2 + mn = m^2 \cos\theta + mn \qty(\frac{\cos\theta}{2}
+ \frac{\sqrt{3} \sin\theta}{2}).
\end{cases}
$$

Summing the two equations above gives us
\begin{equation} \label{eq:costheta}
\boxed{\cos\theta = \frac{1}{2} \cdot \frac{m^2 + n^2 + 4mn}{m^2 + n^2 + mn}.}
\end{equation}


\pagebreak

\section{Moiré pattern}

By taking the norm of $\vb{L}_1$ from equation \ref{eq:L1} and using the angle relation in equation \ref{eq:costheta}, we find that the superlattice constant $L = \abs{\vb{L}_1} = \abs{\vb{L}_2}$ is given by
$$
2\sin[2](\theta/2) = 1 - \cos\theta = \frac{(m-n)^2}{2(m^2+n^2+mn)} \implies
\sqrt{m^2+n^2+mn} = \frac{\abs{m-n}}{2\sin(\theta/2)} \implies
$$
\begin{equation} \label{eq:}
L = a\sqrt{m^2 + n^2 + mn} = \frac{\abs{m-n}}{2 \sin(\theta/2)} \, a.
\end{equation}

\n


The area of an unit cell of the superlattice é $A = \frac{\sqrt{3}}{2} L^2 = (m^2 + n^2 + mn) \, A_1$, where $A_1 = \frac{\sqrt{3}}{2} \, a^2$ is the area of unit cell of monolayer graphene. If we consider now the area of the Brillouin Zone, we get
\begin{equation} \label{eq:bz-volume}
\Omega = \frac{\Omega_1}{m^2 + n^2 + mn},
\end{equation}
where $\Omega_1 = (2\pi)^2/A$ is the BZ area of the monolayer and $\Omega$ is the area of the moiré mini BZ.

\n

For example, $(m,n) = (1,2)$ and $\theta = 21.8^\circ$ we have $m^2 + n^2 + mn = 7$, therefore the monolayer BZ fits 7 mini BZ's in its area, as we see in Figure \ref{fig:bzminibz}.
\begin{figure}[H]
\centering
\includegraphics[width=0.5\linewidth]{fig/bzminibz.png}
\caption{Monolayers (red and green) and mini BZ's with $(m,n) = (1,2)$ and $\theta = 21.8^\circ$. Taken from \cite{koshino2012}.}
\label{fig:bzminibz}
\end{figure}

\n

\textbf{WHY DO WE ONLY CONSIDERER $\abs{m-n} = 1$?}

\pagebreak

\section{BM Model}

Here we will review the Bistritzer-MacDonald (BM) model \cite{macdonald2011}. First of all, the moiré pattern can be interpreted by a beat effect. Define the functions $h_\ell(\r)$, for each layer $\ell = 1, 2$, that describe their periodicity
$$
h_\ell(\r) = \sum_{k=1}^{3} \cos(\vb{G}_{\ell,k} \vdot \r),
$$
where the wave vectors $\vb{G}_{\ell,1} = \vb{b}_{\ell,1}$, $\vb{G}_{\ell,2} = \vb{b}_{\ell,2}$ and $\vb{G}_{\ell,3} = \vb{b}_{\ell,1} - \vb{b}_{\ell,2}$ give the directions for nearest neightbor hoppings in the hexagonal lattice. The moiré pattern will then be an interference between $h_1(\r)$ and $h_2(\r)$,
$$
h_{\text{moiré}}(\r) = h_1(\r) + h_2(\r) =
\sum_{k=1}^{3}
\, 2 \cos(\frac{\vb{G}_{1,k}+\vb{G}_{2,k}}{2} \vdot \r) \cos(\frac{\vb{G}_{1,k}-\vb{G}_{2,k}}{2} \vdot \r).
$$

The moiré pattern oscillates with $\vb{b}_k^{\text{moiré}} = \vb{G}_{1,k} - \vb{G}_{2,k}$, \cite{handbook2019}.

\n

Working on a coordinate system where the layer 2 is rotated by $\theta/2$ and layer 1 by $-\theta/2$, we have
$$
\vb{b}_1^{\text{moiré}} = \sqrt{3} \abs{\Delta \K} \qty(\frac{1}{2}, -\frac{\sqrt{3}}{2}), \quad
\textcolor{red}{\vb{b}_2^{\text{moiré}} = \sqrt{3} \abs{\Delta \K} \qty(\frac{1}{2}, -\frac{\sqrt{3}}{2}),}
$$
where $\abs{\Delta \K} = 2 \abs{\K} \sin(\theta/2)$ and $\abs{\K} = 4\pi/(3\sqrt{3} d)$.

The area of the moiré lattice unit cell is
$$
A_{\text{moiré}} = \frac{(2\pi)^2}{\abs{\b_1^{\text{moiré}} \cross \b_2^{\text{moiré}}}} = \frac{3\sqrt{3} d^2}{8 \sin[2](\theta/2)}.
$$

\subsection{Hamiltonian}

Our starting point will be a tight-binding model
$$
H = H_1 + H_2 + H_{\perp},
$$
where $H_\ell$ is the hamiltonian of the layer $\ell$, and $H_\perp = V_{12} + V_{12}^\d$ describes the interlayer hybridization. Working with a tight-binding model, it is natural to write this hamiltonian in terms of Bloch waves (\textcolor{red}{mencionar $\vtau_{\ell,\alpha}$ antes})
$$
\ket{\psi_{\ell, \k, \alpha}} = \frac{1}{\sqrt{N_\ell}} \sum_{\R_\ell} e^{i \k \vdot (\R_\ell + \vtau_{\ell,\alpha})} \ket{\ell, R_\ell, \alpha},
$$
where $\ell$ labels the layer, $N_\ell$ is the number of unit cells of layer $\ell$, $\R_\ell$ are the positions of lattice sites, $\vtau_{\ell,\alpha}$ are the orbital centers in the unit cell of each layer, and $\ket{\ell,\R_\ell,\alpha}$ are localized Wannier states. In this basis, considering only nearest-neighbor intralayer hopping, the hamiltonian of each layer is given by
$$
H_\ell(\k) =
\begin{pmatrix}
0 & -t f_\ell(\k) \\
-t f_\ell(\k) & 0
\end{pmatrix},
$$
with $f_\ell(\k) = \sum_{i=1}^{3} e^{i\k \vdot \vdelta_\ell}$.

Planning to describe the low energy states, we write $\k = \pm \K_\ell + \q$, where $\pm \K_\ell$ are the Dirac points of each layer. Expanding to first-order in $\q$, the low-energy hamiltonian is
$$
H^{\pm \K}(\q) = \hbar v_F \abs{\q}
\begin{pmatrix}
0 & e^{\mp i (\theta_\q - \theta_\ell)} \\
e^{\pm i (\theta_\q - \theta_\ell)} & 0
\end{pmatrix}
$$
<++>

\subsection{Interlayer hamiltonian}

The tight-binding interlayer Hamiltonian in second quantization reads
$$
V_{12} = \sum_{\R_1,\alpha,\R_2,\beta} c_{1,\alpha}^\d t_{12}^{\alpha\beta}(\R_1,\R_2) c_{2,\beta}(\R_2),
$$
where
$$
t_{12}^{\alpha\beta}(\R_1,\R_2) =
\mel{1,\R_1,\alpha}{V_{12}}{2,\R_2,\beta}
$$
is the interlayer hopping. Performing the Fourier transformation,
$$
c_{\ell,\alpha}^\d(\R_\ell) = \frac{1}{\sqrt{N_\ell}} \sum_{\k_\ell}
e^{-i\k_\ell \vdot (\R_\ell + \vtau_{\ell,\alpha})} c_{\ell,\alpha}^\d(\k_\ell),
$$
with the sum of $\k_\ell$ over the BZ of layer $\ell$, we have
$$
V_{12} = \sum_{\k_1,\alpha,\k_2,\beta} c_{1,\alpha}^\d(\k_1) T_{12}^{\alpha\beta}(\k_1,\k_2) c_{2,\beta}(\k_2),
$$
where we define
$$
T_{12}^{\alpha\beta}(\k_1,\k_2) =
\frac{1}{\sqrt{N_1 N_2}} \sum_{\R_1,\R_2} e^{-i\k_1\vdot(\R_1+\vtau_{1,\alpha})}
t_{12}^{\alpha\beta}(\R_1,\R_2) e^{i\k_2\vdot(\R_2+\vtau_{2,\beta})}.
$$

Now we assume that the interlayer hopping $t_{12}^{\alpha\beta}(\R_1,\R_2)$ is only a function of the separation between the centers of the two orbitals:
$$
t_{12}^{\alpha\beta}(\R_1,\R_2) = t_{12}^{\alpha\beta}(\R_1+\vtau_{1,\alpha}-\R_2-\vtau_{2,\beta}).
$$

We can then write the Fourier transform,
$$
t_{12}^{\alpha\beta}(\R_1+\vtau_{1,\alpha}-\R_2-\vtau_{2,\beta}) =
\int \frac{\dd[2]{\p}}{(2\pi)^2} e^{i \p \vdot (\R_1+\vtau_{1,\alpha}-\R_2-\vtau_{2,\beta})} t_{12}^{\alpha\beta}(\p).
$$

We have
$$
T_{12}^{\alpha\beta}(\k_1,\k_2) = \frac{1}{\sqrt{N_1 N_2}} \int \frac{\dd[2]{\p}}{(2\pi)^2}
\sum_{\R_1} e^{-i(\k_1-\p)\vdot(\R_1+\vtau_{1,\alpha})} t_{12}^{\alpha\beta}(\p)
\sum_{\R_2} e^{i(\k_2-\p)\vdot(\R_2+\vtau_{2,\beta})} =
$$
$$
= \sqrt{N_1 N_2} \int \frac{\dd[2]{\p}}{(2\pi)^2}
\sum_{\G_1, \G_2} e^{-i\G_1\vdot\vtau_{1,\alpha}} t_{12}^{\alpha\beta}(\p)
e^{i\G_2\vdot\vtau_{2,\beta}} \delta_{\k_1-\p,\G_1} \delta_{\k_2-\p,\G_2},
$$
where we have used the relation $\sum_{\R_\ell} e^{i\k\vdot\R_\ell} = N_\ell \sum_{\G_\ell} \delta_{\k,\G_\ell}$. By elementary Dirac delta properties and \textcolor{red}{substituting $\G_\ell \to -\G_\ell$}, we obtain
$$
T_{12}^{\alpha\beta}(\k_1,\k_2) = \frac{\sqrt{N_1 N_2}}{A}
\sum_{\G_1, \G_2} \textcolor{red}{e^{i\G_1\vdot\vtau_{1,\alpha}}} t_{12}^{\alpha\beta}(\p)
\textcolor{red}{e^{-i\G_2\vdot\vtau_{2,\beta}}} \delta_{\k_1+\G_1, \k_2+\G_2}.
$$

Remembering that $A = A_{u.c.1} N_1 = A_{u.c.2} N_2$, we get
$$
T_{12}^{\alpha\beta}(\k_1,\k_2) = \frac{1}{\sqrt{A_{u.c.1} A_{u.c.2}}}
\sum_{\G_1, \G_2} \textcolor{red}{e^{i\G_1\vdot\vtau_{1,\alpha}}} t_{12}^{\alpha\beta}(\p)
\textcolor{red}{e^{-i\G_2\vdot\vtau_{2,\beta}}} \delta_{\k_1+\G_1, \k_2+\G_2}.
$$

The conservation
$$
\k_1 + \G_1 = \k_2 + \G_2
$$
is known as generalized umklapp condition.

\n

Now we try to guess the behavior of $t_{12}(\r)$. We often see in the literature the estimate in terms of Slater-Koster parameters $V_{pp\s}$ and $V_{pp\pi}$, where they are assumed to exponentially decay. Making some rought estimates, they conclude that $t_\perp(\p)$ is only a function of $\abs{\p}$ and decays very rapidly as $\abs{\p}$ increases.

\begin{figure}[H]
\centering
\includegraphics[width=0.6\linewidth]{fig/tperp.png}
\caption{Fourier transform for the interlayer hopping in tBLG. The vertical dashed line marks the position
of the Dirac point. Taken from \cite{handbook2019}.}
\label{fig:tperp}
\end{figure}

\subsection{Small rotation limit}

<++>






%%-----
%% Referências bibliográficas
%%-----
\addcontentsline{toc}{chapter}{\bibname}
%\bibliographystyle{abntex2-num}
\bibliography{citations}
\bibliographystyle{ieeetr}


\end{document}
